Thesis/210lecture.lean
@@ -1,0 +1,167 @@
+import Lean
+import Mathlib.Data.Real.Basic
+import Mathlib.Data.Matrix.Basic
+import Mathlib.Tactic
+
+-- Part 1 : What is formalization, and why should I care?
+
+
+-- Part 2: What is Lean, and how do I use it?
+
+-- Lean as a proof assistant
+
+-- First order logic
+variable {α β : Type} (P Q : α → Prop) (R : α → β → Prop)
+
+section
+
+theorem ex1 : (∀ x, P x) ∧ (∀ x, Q x) → ∀ x, P x ∧ Q x := by
+  intro h x
+  -- rcases with ⟨hp, hq⟩
+  constructor
+  . have lol : ∀ (x : α), P x := by exact h.left
+    exact lol x
+  . have lol : ∀ (x : α), Q x := by exact h.right
+    exact lol x
+
+theorem ex2 : (∀ x, P x) ∨ (∀ x, Q x) → ∀ x, P x ∨ Q x := by
+  sorry
+
+theorem ex3 : (∃ x, ∀ y, R x y) → ∀ y, ∃ x, R x y := by
+  sorry
+
+end
+
+variable (P Q R S : Prop)
+
+example (h1 : P ∨ Q) (h2 : P → R) : R ∨ Q := by sorry
+
+
+-- this one requires classical logic!
+example (h : ¬ (P ∧ Q)) : ¬ P ∨ ¬ Q := by sorry
+
+
+
+-- More induciton
+
+section
+variable {α : Type*} [CommMonoid α]
+
+def mypow : α → ℕ → α
+  | a, 0       => 1
+  | a, (n + 1) => a * (mypow a n)
+
+
+theorem mypow_zero (a : α) : mypow a 0 = 1 := rfl
+
+theorem mypow_succ (a : α) (n : ℕ) : mypow a (n + 1) = a * mypow a n := rfl
+
+theorem mypow_add (a : α) (m n : ℕ) : mypow a (m + n) = mypow a m * mypow a n := by
+  sorry
+
+end
+
+
+
+
+
+
+
+
+
+
+-- Part 3: 15-150 and 15-210 reloaded, Lean as a verifiable programming language
+
+-- Structural induction
+
+-- The following is an inductive definition of binary trees:
+inductive BinTree where
+  | empty : BinTree
+  | node : BinTree → BinTree → BinTree
+
+namespace BinTree
+
+/-
+We can define the size and the depth of a binary tree
+by recursion.
+-/
+
+def size : BinTree → ℕ
+  | BinTree.empty => 0
+  | BinTree.node l r => size l + size r + 1
+
+def depth : BinTree → ℕ
+  | BinTree.empty => 0
+  | BinTree.node l r => max (depth l) (depth r) + 1
+
+def flip : BinTree → BinTree
+  | empty => empty
+  | node l r => node (flip r) (flip l)
+
+theorem size_flip : ∀ t, size (flip t) = size t := by
+  intro t
+  induction t with
+  | empty => rw [flip]
+  | node l r ihL ihR => rw [flip, size, size, ihL, ihR]; omega
+
+theorem depth_le_size : ∀ t : BinTree, depth t ≤ size t := by
+  intro t
+  induction t with
+  | empty => rw [depth, size]
+  | node l r ihl ihr =>
+      rw [depth, size, add_le_add_iff_right]
+      rcases max_cases l.depth r.depth with hl | hr
+      . rw [hl.left]
+        apply le_add_right
+        exact ihl
+      . rw [hr.left]
+        apply le_add_left
+        exact ihr
+
+
+
+
+
+
+
+
+
+section
+open List
+
+example (f : α → β) (xs : List α) : map f (tail xs) = tail (map f xs) := by
+  induction xs with
+  | nil => rw [tail, map, tail]
+  | cons a l _ => rw [tail, map, tail]
+
+def snoc : List α → α → List α
+  | [], y => [y]
+  | (x :: xs), y => x :: snoc xs y
+
+-- You use these:
+#check nil_append
+#check cons_append
+
+-- 4C. Prove this.
+theorem snoc_eq_append (xs : List α) (y : α) : snoc xs y = xs ++ [y] := by
+  induction xs with
+  | nil => rw [snoc, nil_append]
+  | cons a l ih => rw [snoc, cons_append, ih]
+
+-- 4D. Prove this by induction.
+theorem map_snoc (f : α → β) (xs : List α) (y : α) : map f (snoc xs y) = snoc (map f xs) (f y) := by
+  sorry
+
+#check map_append
+
+-- 4E. Prove it again without induction, using `snoc_eq_apppend` and `map_append`.
+theorem map_snoc' (f : α → β) (xs : List α) (y : α) : map f (snoc xs y) = snoc (map f xs) (f y) := by
+  sorry
+
+end
+
+-- open Finset
+-- -- Proof over finite sets
+
+-- theorem ex4 (x : ℝ) (n : ℕ) : (∑ i in range n, x^i) * (x - 1) = x^n - 1 := by
+--   sorry
